src/PROBABLY_ALGO.v
@@ -1,0 +1,132 @@
+Require Import MC_CTL.
+Require Import List. Import ListNotations.
+Require Import Lia.
+
+Ltac SOLVE_AX2' init_l solve_subformula1 := let next_state := fresh "next_state" in 
+intro next_state;
+let trans_to_new_state := fresh "trans_to_new_state" in 
+intro trans_to_new_state;
+compute in trans_to_new_state;
+repeat (
+  let a := fresh "a" in
+  let b := fresh "b" in
+  destruct trans_to_new_state as (a&b);
+  ((apply a in init_l)+(apply b in init_l));
+  (
+    lazymatch type of init_l with 
+    | _ \/ _ => (repeat destruct init_l as [init_l|init_l])
+    | _ => idtac
+    end
+  ));
+  solve_subformula1 init_l.
+
+
+Ltac SOLVE_AU2' n max_of_state init_l solve_subformula1 solve_subformula2 := 
+let solve_AU max_of_state :=
+    let path_pi := fresh "path_pi" in
+    intro path_pi;
+    let is_path_pi := fresh "is_path_pi" in
+    intro is_path_pi;
+    let first_state:= fresh "first_state" in
+    intro first_state;
+    compute;
+    let (*rec*) sol_AU n :=
+    (* tryif (let h:= fresh "h" in assert(h: n <= max_of_state); [progress auto | auto])
+    then *)
+    (
+        eexists n (*n*); 
+        [
+            auto;
+            let m := fresh "m" in
+            let le_m := fresh "le_m" in
+            intro m;
+            intro le_m;
+            (
+            let rec solve_rec le_m := 
+                apply usefull in le_m; (*compute in le_m;*)
+                destruct le_m as [ le_m | le_m];
+                [>
+                apply usefull2 in le_m;
+                rewrite init_l in first_state;
+                let rec loop_to_needed_m i m :=
+                    tryif (let h:= fresh "h" in assert(h: i < m); [progress auto | auto])
+                    then 
+                        let is_path_pi_i := fresh "is_path_pi_i" in
+                        pose proof (is_path_pi i) as is_path_pi_i;
+                        compute in is_path_pi_i;
+                        repeat (
+                            let a := fresh "a" in
+                            let b := fresh "b" in
+                            destruct is_path_pi_i as (a&b);
+                            ((apply a in first_state)+(apply b in first_state));
+                            (
+                            lazymatch type of first_state with 
+                            | _ \/ _ => (repeat destruct first_state as [first_state|first_state])
+                            | _ => idtac
+                            end
+                            );
+                            loop_to_needed_m (i + 1) m)
+                    else 
+                        idtac
+                in
+                lazymatch type of le_m with 
+                | _ = ?k => loop_to_needed_m 0 k
+                | _ => idtac
+                end
+                ;
+                rewrite <- le_m in first_state;
+                solve_subformula1 first_state
+                
+                | 
+                lia +  
+                (solve_rec le_m) + auto
+                ]
+            in
+            (solve_rec le_m)
+            )
+            
+        |
+        rewrite init_l in first_state;
+        let rec loop_to_needed_m i m :=
+            tryif (let h:= fresh "h" in assert(h: i < m); [progress auto | auto])
+            then 
+                let is_path_pi_i := fresh "is_path_pi_i" in
+                pose proof (is_path_pi i) as is_path_pi_i;
+                compute in is_path_pi_i;
+                repeat (
+                    let a := fresh "a" in
+                    let b := fresh "b" in
+                    destruct is_path_pi_i as (a&b);
+                    ((apply a in first_state)+(apply b in first_state));
+                    (
+                    lazymatch type of first_state with 
+                    | _ \/ _ => (repeat destruct first_state as [first_state|first_state])
+                    | _ => idtac
+                    end
+                    );
+                    loop_to_needed_m (i + 1) m)
+            else 
+                fail "loop_to_needed_m"
+        in
+        loop_to_needed_m 0 2;
+        solve_subformula2 first_state
+        ]
+    )
+    (* +
+    sol_AU (n + 1)
+    else 
+    fail "solve_AU: with" n*)
+    in 
+    sol_AU n
+in
+solve_AU max_of_state .
+
+
+
+Ltac SOLVE_FV' init_l := (*solve satisfies model (fV ?) (?st) problem *)
+  repeat split;
+  let pre := fresh "pre" in
+  intro pre; 
+  rewrite init_l in pre; 
+  discriminate
+.
